Rename eval -> accepts

BoltLean/Ltl.lean
@@ -18,33 +18,33 @@ deriving DecidableEq
 
 namespace Formula
 
-  def eval (phi: Formula n) (t: Trace n): Prop :=
+  def accepts (phi: Formula n) (t: Trace n): Prop :=
   match t with
     | .nil => match phi with
       | True | WeakNext _ | Globally _ => _root_.True
       | False | Finally _ | Var _ _ | Next _ |  Until _ _ => _root_.False
-      | Or psi1 psi2 => (eval psi1 t) ∨ (eval psi2 t)
-      | And psi1 psi2 => (eval psi1 t) ∧ (eval psi2 t)
+      | Or psi1 psi2 => (accepts psi1 t) ∨ (accepts psi2 t)
+      | And psi1 psi2 => (accepts psi1 t) ∧ (accepts psi2 t)
     | head::tail => match phi with
       | True => _root_.True
       | False => _root_.False
       | Var v neg => xor head[v] neg
-      | Next psi => eval psi tail
-      | WeakNext psi => tail = List.nil ∨ eval psi tail
-      | Globally psi => ∀ j, j < t.length → eval psi (t.drop j)
-      | Finally psi => ∃ j, j < t.length ∧ eval psi (t.drop j)
-      | Or psi1 psi2 => (eval psi1 t) ∨ (eval psi2 t)
-      | And psi1 psi2 => (eval psi1 t) ∧ (eval psi2 t)
+      | Next psi => accepts psi tail
+      | WeakNext psi => tail = List.nil ∨ accepts psi tail
+      | Globally psi => ∀ j, j < t.length → accepts psi (t.drop j)
+      | Finally psi => ∃ j, j < t.length ∧ accepts psi (t.drop j)
+      | Or psi1 psi2 => (accepts psi1 t) ∨ (accepts psi2 t)
+      | And psi1 psi2 => (accepts psi1 t) ∧ (accepts psi2 t)
       | Until psi1 psi2 => ∃ j, j < t.length ∧
-                                (eval psi2 (t.drop j)) ∧
-                                (∀ k, k < j → eval psi1 (t.drop k))
+                                (accepts psi2 (t.drop j)) ∧
+                                (∀ k, k < j → accepts psi1 (t.drop k))
 
-  def equivalence (phi psi : Formula n) : Prop := ∀ (t : Trace n), eval phi t ↔ eval psi t
+  def equivalence (phi psi : Formula n) : Prop := ∀ (t : Trace n), accepts phi t ↔ accepts psi t
 
   theorem congruence_finally (phi1 phi2 : Formula n) :
   (equivalence phi1 phi2) → equivalence (Finally phi1) (Finally phi2) := by
   intro h1 h2
-  unfold eval
+  unfold accepts
   simp
   match h2 with
     | List.nil => simp
@@ -61,7 +61,7 @@ namespace Formula
   theorem congruence_globally (phi1 phi2 : Formula n) :
   (equivalence phi1 phi2) → equivalence (Globally phi1) (Globally phi2) := by
   intro h1 h2
-  unfold eval
+  unfold accepts
   simp
   match h2 with
     | List.nil => simp
@@ -72,65 +72,5 @@ namespace Formula
                         first | rw [h1] | rw [←h1]
                         apply h
                       )
-
-
-
-
-  theorem congruence (phi1 psi1 phi2 psi2 : Formula n) :
-    (equivalence phi1 phi2) → (equivalence psi1 psi2) → equivalence (Until phi1 psi1) (Until phi2 psi2) := by
-      unfold equivalence
-      intro h1 h2
-      sorry
-
-
-
-  theorem simplification_rule (phi : Formula n) : equivalence (Finally (Finally phi)) (Finally phi) := by sorry
-
-
-  -- theorem or_eval (phi psi: Formula n) (t: Trace n):
-  --   (phi.Or psi).eval t ↔ phi.eval t ∨ psi.eval t  := by
-  --     constructor
-  --     . intro h
-  --       simp [eval, eval_aux] at h
-  --       by_cases htl: 0 < t.length
-  --       . simp [htl] at h
-  --         unfold eval
-  --         simp [htl]
-  --         exact h
-  --       . simp [htl] at h
-  --         assumption
-  --     . intro h
-  --       rw [eval]
-  --       by_cases htl: 0 < t.length
-  --       all_goals simp [htl]
-  --       . unfold eval at h
-  --         simp [htl] at h
-  --         rw [eval_aux]
-  --         assumption
-  --       . exact h
-
-
-  -- theorem and_eval (phi psi: Formula n) (t: Trace n):
-  --   (phi.And psi).eval t ↔ phi.eval t ∧ psi.eval t  := by
-  --     constructor
-  --     . intro h
-  --       simp [eval, eval_aux] at h
-  --       by_cases htl: 0 < t.length
-  --       . simp [htl] at h
-  --         unfold eval
-  --         simp [htl]
-  --         exact h
-  --       . simp [htl] at h
-  --         assumption
-  --     . intro h
-  --       rw [eval]
-  --       by_cases htl: 0 < t.length
-  --       all_goals simp [htl]
-  --       . unfold eval at h
-  --         simp [htl] at h
-  --         rw [eval_aux]
-  --         assumption
-  --       . exact h
-
 
 end Formula
